### The Pythagorean identity
  
$$ \sin^2y+\cos^2y=1 $$
$$ \cos^2y=1-\sin^2y $$
$$ \cos\left(y\right)=\sqrt{1-\sin^2y} $$
$$ \sin^2y=1-\cos^2\left(y\right) $$
$$ \sin\left(y\right)=\sqrt{1-\cos^2\left(y\right)} $$


### Derivative of inverse sine

$$ y=\sin^{-1}x $$
$$ \sin\left(y\right)=x $$
$$ \frac{d}{dx}\left\lbrack\sin\left(y\right)\right\rbrack=\frac{d}{dx}\left\lbrack x\right\rbrack $$
$$ \cos\left(y\right)\cdot\frac{dy}{dx}=1 $$
$$ \frac{dy}{dx}=\frac{1}{\cos\left(y\right)} $$
Hence the trig identity above (Pythagorean)
$$ \frac{dy}{dx}=\frac{1}{\sqrt{1-\left(\sin^{}y\right)^2}} $$
Now remember `sin(y)=x`, first step above, and we substitute x
$$ \frac{dy}{dx}=\frac{1}{\sqrt{1-x^2}} $$



### Derivative of inverse cosine
$$ y=\cos^{-1}x $$
$$ x=\cos\left(y\right) $$
$$ \frac{d}{dx}\left\lbrack x\right\rbrack=\frac{d}{dx}\left\lbrack\cos y\right\rbrack $$
$$ 1=-\sin\left(y\right)\cdot\frac{dy}{dx} $$
$$ \frac{dy}{dx}=\frac{-1}{\sin\left(y\right)} $$
Hence the trig identity above (Pythagorean)
$$ \frac{dy}{dx}=\frac{-1}{\sqrt{1-\cos^{}\left(y\right)^2}} $$
Now remember `cos(y)=x`, first step above, and we substitute x
$$ \frac{dy}{dx}=\frac{-1}{\sqrt{1-x^2}} $$