### Definition of an inverse function

$$ \Huge g\left(x\right)=f^{-1}\left(x\right) $$

```
$$ g\left(x\right)=f^{-1}\left(x\right) $$
```

#### In respect to (x)

$$ \Huge g\left(f\left(x\right)\right)=x $$

```
$$ g\left(f\left(x\right)\right)=x $$
```

### Now taking derivative of both sides

$$ \Huge \frac{d}{dx}\left\lbrack g\left(f\left(x\right)\right)\right\rbrack=\frac{d}{dx}\left\lbrack x\right\rbrack $$

```
$$  \frac{d}{dx}\left\lbrack g\left(f\left(x\right)\right)\right\rbrack=\frac{d}{dx}\left\lbrack x\right\rbrack $$
```

### Applying the chain rule

$$ \Huge g^{\prime}\left(f\left(x\right)\right)\cdot f^{\prime}\left(x\right)=1 $$

```
$$ g^{\prime}\left(f\left(x\right)\right)\cdot f^{\prime}\left(x\right)=1 $$
```

### The final derivative

In respect to f'(x)
$$ \Huge f^{\prime}\left(x\right)=\frac{1}{g^{\prime}\left(f\left(x\right)\right)} $$

```
$$ f^{\prime}\left(x\right)=\frac{1}{g^{\prime}\left(f\left(x\right)\right)} $$
```

in Respect to g'(x)

$$ g^{\prime}\left(x\right)=\frac{1}{f^{\prime}\left(g\left(x\right)\right)} $$
```
$$ g^{\prime}\left(x\right)=\frac{1}{f^{\prime}\left(g\left(x\right)\right)} $$
```